revive header_decrypt_ct; skeleton for Impl.header_decrypt_aux

src/QUIC.Impl.Header.fst
@@ -3,7 +3,8 @@ friend QUIC.Spec.Header
 
 open QUIC.Impl.Header.Base
 
-module ParseSpec = QUIC.Spec.Header.Parse
+module Parse = QUIC.Spec.Header.Parse
+module ParseImpl = QUIC.Impl.Header.Parse
 module Spec = QUIC.Spec.Header
 module PN = QUIC.Spec.PacketNumber.Base
 
@@ -24,6 +25,9 @@ module SecretBuffer = QUIC.Secret.Buffer
 module Lemmas = QUIC.Impl.Lemmas
 module BF = LowParse.BitFields
 
+module SCipher = Spec.Agile.Cipher
+module SAEAD = Spec.Agile.AEAD
+
 (* There are a few places where EverCrypt needs public data whereas it
 could/should be secret. Thus, we may need some declassification
 locally using Lib.RawIntTypes, but we definitely don't want to make
@@ -31,15 +35,15 @@ secret integers globally transparent using friend *)
 
 module ADMITDeclassify = Lib.RawIntTypes
 
-let block_len (a: Spec.Agile.Cipher.cipher_alg):
-  x:U32.t { U32.v x = Spec.Agile.Cipher.block_length a }
+let block_len (a: SCipher.cipher_alg):
+  x:U32.t { U32.v x = SCipher.block_length a }
 =
-  let open Spec.Agile.Cipher in
+  let open SCipher in
   match a with | CHACHA20 -> 64ul | _ -> 16ul
 
 #push-options "--z3rlimit 256"
 inline_for_extraction
-let block_of_sample (a: Spec.Agile.Cipher.cipher_alg)
+let block_of_sample (a: SCipher.cipher_alg)
   (dst: B.buffer Secret.uint8)
   (s: CTR.state a)
   (k: B.buffer Secret.uint8)
@@ -50,8 +54,8 @@ let block_of_sample (a: Spec.Agile.Cipher.cipher_alg)
       CTR.invariant h0 s /\
       B.(all_disjoint
         [ CTR.footprint h0 s; loc_buffer dst; loc_buffer k; loc_buffer sample ]) /\
-      Spec.Agile.Cipher.(a == AES128 \/ a == AES256 \/ a == CHACHA20) /\
-      B.length k = Spec.Agile.Cipher.key_length a /\
+      SCipher.(a == AES128 \/ a == AES256 \/ a == CHACHA20) /\
+      B.length k = SCipher.key_length a /\
       B.length dst = 16 /\
       B.length sample = 16)
     (ensures fun h0 _ h1 ->
@@ -68,7 +72,7 @@ let block_of_sample (a: Spec.Agile.Cipher.cipher_alg)
   let dst_block' = B.alloca (Secret.to_u8 0uy) 64ul in
   let dst_block = B.sub dst_block' 0ul (block_len a) in
   begin match a with
-  | Spec.Agile.Cipher.CHACHA20 ->
+  | SCipher.CHACHA20 ->
       let ctr = SecretBuffer.load32_le (B.sub sample 0ul 4ul) in
       let iv = B.sub sample 4ul 12ul in
       (**) let h1 = HST.get () in
@@ -78,12 +82,12 @@ let block_of_sample (a: Spec.Agile.Cipher.cipher_alg)
       CTR.update_block (G.hide a) s dst_block zeroes;
       (**) let h2 = HST.get () in
       (**) Lemmas.seq_map2_xor0 (B.as_seq h1 dst_block)
-      (**)   (Spec.Agile.Cipher.ctr_block a (B.as_seq h0 k) (B.as_seq h1 iv) (Secret.v ctr));
+      (**)   (SCipher.ctr_block a (B.as_seq h0 k) (B.as_seq h1 iv) (Secret.v ctr));
       (**) assert (B.as_seq h2 dst_block `Seq.equal`
-      (**)   Spec.Agile.Cipher.ctr_block a (B.as_seq h0 k) (B.as_seq h1 iv) (Secret.v ctr));
+      (**)   SCipher.ctr_block a (B.as_seq h0 k) (B.as_seq h1 iv) (Secret.v ctr));
       let dst_slice = B.sub dst_block 0ul 16ul in
       (**) assert (B.as_seq h2 dst_slice `Seq.equal` Seq.slice (
-      (**)   Spec.Agile.Cipher.ctr_block a (B.as_seq h0 k) (B.as_seq h1 iv) (Secret.v ctr)
+      (**)   SCipher.ctr_block a (B.as_seq h0 k) (B.as_seq h1 iv) (Secret.v ctr)
       (**) ) 0 16);
       B.blit dst_slice 0ul dst 0ul 16ul
   | _ ->
@@ -96,12 +100,12 @@ let block_of_sample (a: Spec.Agile.Cipher.cipher_alg)
       CTR.update_block (G.hide a) s dst_block zeroes;
       (**) let h2 = HST.get () in
       (**) Lemmas.seq_map2_xor0 (B.as_seq h1 dst_block)
-      (**)   (Spec.Agile.Cipher.ctr_block a (B.as_seq h0 k) (B.as_seq h1 iv) (Secret.v ctr));
+      (**)   (SCipher.ctr_block a (B.as_seq h0 k) (B.as_seq h1 iv) (Secret.v ctr));
       (**) assert (B.as_seq h2 dst_block `Seq.equal`
-      (**)   Spec.Agile.Cipher.ctr_block a (B.as_seq h0 k) (B.as_seq h1 iv) (Secret.v ctr));
+      (**)   SCipher.ctr_block a (B.as_seq h0 k) (B.as_seq h1 iv) (Secret.v ctr));
       let dst_slice = B.sub dst_block 0ul 16ul in
       (**) assert (B.as_seq h2 dst_slice `Seq.equal` Seq.slice (
-      (**)   Spec.Agile.Cipher.ctr_block a (B.as_seq h0 k) (B.as_seq h1 iv) (Secret.v ctr)
+      (**)   SCipher.ctr_block a (B.as_seq h0 k) (B.as_seq h1 iv) (Secret.v ctr)
       (**) ) 0 16);
       B.blit dst_slice 0ul dst 0ul 16ul
   end;
@@ -129,21 +133,21 @@ let index_pn_sizemask_ct_right
 
 let header_encrypt_ct
   (a:ea)
-  (hpk: Spec.Agile.Cipher.key (Spec.Agile.AEAD.cipher_alg_of_supported_alg a))
+  (hpk: SCipher.key (SAEAD.cipher_alg_of_supported_alg a))
   (h: Spec.header)
   (c: cbytes' (Spec.is_retry h))
 : GTot packet
 = 
   assert_norm(max_cipher_length < pow2 62);
-  let r = ParseSpec.format_header h `Seq.append` c in
+  let r = Parse.format_header h `Seq.append` c in
   if Spec.is_retry h
   then
     r
   else
-    let pn_offset = ParseSpec.pn_offset h in
+    let pn_offset = Parse.pn_offset h in
     let pn_len = Secret.v (Spec.pn_length h) - 1 in
     let sample = Seq.seq_hide (Seq.slice c (3-pn_len) (19-pn_len)) in
-    let mask = Seq.seq_reveal (Spec.block_of_sample (Spec.Agile.AEAD.cipher_alg_of_supported_alg a) hpk sample) in
+    let mask = Seq.seq_reveal (Spec.block_of_sample (SAEAD.cipher_alg_of_supported_alg a) hpk sample) in
     let pnmask = Lemmas.and_inplace (Seq.slice mask 1 5) (pn_sizemask_ct pn_len) 0 in
     let f = Seq.index r 0 in
     let protected_bits = if Spec.MShort? h then 5 else 4 in
@@ -156,21 +160,21 @@ let header_encrypt_ct
 
 let header_encrypt_ct_correct
   (a:ea)
-  (hpk: Spec.Agile.Cipher.key (Spec.Agile.AEAD.cipher_alg_of_supported_alg a))
+  (hpk: SCipher.key (SAEAD.cipher_alg_of_supported_alg a))
   (h: Spec.header)
   (c: cbytes' (Spec.is_retry h))
 : Lemma
   (header_encrypt_ct a hpk h c `Seq.equal` Spec.header_encrypt a hpk h c)
 =
   assert_norm(max_cipher_length < pow2 62);
-  let r = ParseSpec.format_header h `Seq.append` c in
+  let r = Parse.format_header h `Seq.append` c in
   if Spec.is_retry h
   then ()
   else begin
-    let pn_offset = ParseSpec.pn_offset h in
-    let pn_len = Secret.v (ParseSpec.pn_length h) - 1 in
+    let pn_offset = Parse.pn_offset h in
+    let pn_len = Secret.v (Parse.pn_length h) - 1 in
     let sample = Seq.seq_hide (Seq.slice c (3-pn_len) (19-pn_len)) in
-    let mask = Seq.seq_reveal (Spec.block_of_sample (Spec.Agile.AEAD.cipher_alg_of_supported_alg a) hpk sample) in
+    let mask = Seq.seq_reveal (Spec.block_of_sample (SAEAD.cipher_alg_of_supported_alg a) hpk sample) in
     let pnmask_ct = Lemmas.and_inplace (Seq.slice mask 1 5) (pn_sizemask_ct pn_len) 0 in
     let pnmask_naive = Lemmas.and_inplace (Seq.slice mask 1 (pn_len + 2)) (Spec.pn_sizemask pn_len) 0 in
     Lemmas.pointwise_op_split U8.logand (Seq.slice mask 1 5) (pn_sizemask_ct pn_len) 0 (pn_len + 1);
@@ -194,17 +198,17 @@ let header_encrypt_ct_correct
 
 let header_encrypt_ct_secret_preserving_not_retry_spec
   (a:ea)
-  (hpk: Spec.Agile.Cipher.key (Spec.Agile.AEAD.cipher_alg_of_supported_alg a))
+  (hpk: SCipher.key (SAEAD.cipher_alg_of_supported_alg a))
   (h: Spec.header { ~ (Spec.is_retry h) })
   (r: Seq.seq Secret.uint8 {
-    Seq.length r >= ParseSpec.pn_offset h + 20
+    Seq.length r >= Parse.pn_offset h + 20
   })
 : GTot (Seq.seq Secret.uint8)
 = 
-  let pn_offset = ParseSpec.pn_offset h in
+  let pn_offset = Parse.pn_offset h in
   let pn_len = Secret.v (Spec.pn_length h) - 1 in
   let sample = (Seq.slice r (pn_offset + 4) (pn_offset + 20)) in
-  let mask = (Spec.block_of_sample (Spec.Agile.AEAD.cipher_alg_of_supported_alg a) hpk sample) in
+  let mask = (Spec.block_of_sample (SAEAD.cipher_alg_of_supported_alg a) hpk sample) in
   let pnmask = Lemmas.secret_and_inplace (Seq.slice mask 1 5) (Seq.seq_hide (pn_sizemask_ct pn_len)) 0 in
   let f = Seq.index r 0 in
   let protected_bits = if Spec.MShort? h then 5ul else 4ul in
@@ -219,7 +223,7 @@ let header_encrypt_ct_secret_preserving_not_retry_spec
 
 let header_encrypt_ct_secret_preserving_not_retry_spec_correct
   (a:ea)
-  (hpk: Spec.Agile.Cipher.key (Spec.Agile.AEAD.cipher_alg_of_supported_alg a))
+  (hpk: SCipher.key (SAEAD.cipher_alg_of_supported_alg a))
   (h: Spec.header)
   (c: cbytes)
 : Lemma
@@ -227,19 +231,19 @@ let header_encrypt_ct_secret_preserving_not_retry_spec_correct
     (~ (Spec.is_retry h))
   ))
   (ensures (
-    let r = ParseSpec.format_header h `Seq.append` c in
-    Seq.length r >= ParseSpec.pn_offset h + 20 /\
+    let r = Parse.format_header h `Seq.append` c in
+    Seq.length r >= Parse.pn_offset h + 20 /\
     Spec.header_encrypt a hpk h c == Seq.seq_reveal (header_encrypt_ct_secret_preserving_not_retry_spec a hpk h (Seq.seq_hide r))
   ))
 = header_encrypt_ct_correct a hpk h c;
-  let fmt = ParseSpec.format_header h in
+  let fmt = Parse.format_header h in
   let len = Seq.length fmt in
   let pr = fmt `Seq.append` c in
-  assert (Seq.length pr >= ParseSpec.pn_offset h + 20);
+  assert (Seq.length pr >= Parse.pn_offset h + 20);
   let pn_len = Secret.v (Spec.pn_length h) - 1 in
   let psample = Seq.slice c (3 - pn_len) (19 - pn_len) in
   assert (c `Seq.equal` Seq.slice pr len (Seq.length pr));
-  let pn_off = ParseSpec.pn_offset h in
+  let pn_off = Parse.pn_offset h in
   assert (pn_off + pn_len + 1 == len);
   assert (c == Seq.slice pr (pn_off + pn_len + 1) (Seq.length pr));
   Seq.slice_slice pr (pn_off + pn_len + 1) (Seq.length pr) (3 - pn_len) (19 - pn_len);
@@ -247,7 +251,7 @@ let header_encrypt_ct_secret_preserving_not_retry_spec_correct
   let r = Seq.seq_hide #Secret.U8 pr in
   let sample = Seq.slice r (pn_off + 4) (pn_off + 20) in
   assert (sample == Seq.seq_hide #Secret.U8 psample);
-  let mask = Spec.block_of_sample (Spec.Agile.AEAD.cipher_alg_of_supported_alg a) hpk sample in
+  let mask = Spec.block_of_sample (SAEAD.cipher_alg_of_supported_alg a) hpk sample in
   let pmask = Seq.seq_reveal mask in
   assert (mask == Seq.seq_hide pmask);
   let mask15 = Seq.slice mask 1 5 in
@@ -319,7 +323,7 @@ let pn_sizemask (dst: B.buffer Secret.uint8) (pn_len: PN.packet_number_length_t)
 
 let header_encrypt_ct_secret_preserving_not_retry
   (a: ea)
-  (s: CTR.state (Spec.Agile.AEAD.cipher_alg_of_supported_alg a))
+  (s: CTR.state (SAEAD.cipher_alg_of_supported_alg a))
   (k: B.buffer Secret.uint8)
   (h: Ghost.erased Spec.header)
   (is_short: bool)
@@ -334,7 +338,7 @@ let header_encrypt_ct_secret_preserving_not_retry
     CTR.invariant m s /\
     B.all_disjoint
       [ CTR.footprint m s; B.loc_buffer k; B.loc_buffer dst] /\
-    B.length k == Spec.Agile.Cipher.key_length (Spec.Agile.AEAD.cipher_alg_of_supported_alg a) /\
+    B.length k == SCipher.key_length (SAEAD.cipher_alg_of_supported_alg a) /\
     (~ (Spec.is_retry h)) /\
     is_short == (Spec.MShort? h) /\
     U32.v pn_offset == Parse.pn_offset h /\
@@ -365,9 +369,9 @@ let header_encrypt_ct_secret_preserving_not_retry
   let m1 = HST.get () in
   let gsample = Ghost.hide (Seq.slice (B.as_seq m0 dst) (U32.v pn_offset + 4) (U32.v pn_offset + 20)) in
   assert (B.as_seq m1 sample == Ghost.reveal gsample);
-  block_of_sample (Spec.Agile.AEAD.cipher_alg_of_supported_alg a) mask s k sample;
+  block_of_sample (SAEAD.cipher_alg_of_supported_alg a) mask s k sample;
   let m2 = HST.get () in
-  let gmask = Ghost.hide (Spec.block_of_sample (Spec.Agile.AEAD.cipher_alg_of_supported_alg a) (B.as_seq m0 k) gsample) in
+  let gmask = Ghost.hide (Spec.block_of_sample (SAEAD.cipher_alg_of_supported_alg a) (B.as_seq m0 k) gsample) in
   assert (B.as_seq m2 mask == Ghost.reveal gmask);
   pn_sizemask pn_sm pn_len;
   let m3 = HST.get () in
@@ -404,7 +408,7 @@ let header_encrypt
   else begin
     let m = HST.get () in
     let hpk = Ghost.hide (B.as_seq m k) in
-    let fmt = Ghost.hide (ParseSpec.format_header (G.reveal h)) in
+    let fmt = Ghost.hide (Parse.format_header (G.reveal h)) in
     let cipher = Ghost.hide (Seq.slice (B.as_seq m dst) (Seq.length fmt)  (B.length dst)) in
     assert (B.as_seq m dst `Seq.equal` (fmt `Seq.append` cipher));
     header_encrypt_ct_secret_preserving_not_retry_spec_correct a hpk h cipher;
@@ -434,6 +438,342 @@ let header_encrypt
   end
 
 #pop-options
+
+
+(* A constant-time specification of header_decrypt_aux which does not test or truncate on pn_len *)
+
+let header_decrypt_aux_ct
+  (a:ea)
+  (hpk: SCipher.key (SAEAD.cipher_alg_of_supported_alg a))
+  (cid_len: nat { cid_len <= 20 })
+  (packet: packet)
+: GTot (option Spec.header_decrypt_aux_t)
+= let open FStar.Math.Lemmas in
+  if Seq.length packet = 0
+  then None
+  else
+    let f = Seq.index packet 0 in
+    let is_short = (BF.get_bitfield (U8.v f) 7 8 = 0) in
+    let is_retry = not is_short && BF.get_bitfield (U8.v f) 4 6 = 3 in
+    if is_retry
+    then
+      Some ({
+        Spec.is_short = is_short;
+        Spec.is_retry = is_retry;
+        Spec.packet = packet;
+        Spec.pn_offset = ();
+        Spec.pn_len = ();
+      })
+    else
+      match Parse.putative_pn_offset cid_len packet with
+      | None -> None
+      | Some pn_offset ->
+        let sample_offset = pn_offset + 4 in
+        if sample_offset + 16 > Seq.length packet
+        then None
+        else begin
+          let sample = Seq.slice packet sample_offset (sample_offset+16) in
+          let mask = Seq.seq_reveal (Spec.block_of_sample (SAEAD.cipher_alg_of_supported_alg a) hpk (Seq.seq_hide sample)) in
+          (* mask the least significant bits of the first byte *)
+          let protected_bits = if is_short then 5 else 4 in
+          let f' = BF.set_bitfield (U8.v f) 0 protected_bits (BF.get_bitfield (U8.v f `FStar.UInt.logxor` U8.v (Seq.index mask 0)) 0 protected_bits) in
+          let packet' = Seq.cons (U8.uint_to_t f') (Seq.slice packet 1 (Seq.length packet)) in
+          (* now the packet number length is available, so mask the packet number *)
+          let pn_len = BF.get_bitfield f' 0 2 in
+          let pnmask = Lemmas.and_inplace (Seq.slice mask 1 5) (pn_sizemask_ct pn_len) 0 in
+          let packet'' = Lemmas.xor_inplace packet' pnmask pn_offset in
+          Some ({
+            Spec.is_short = is_short;
+            Spec.is_retry = is_retry;
+            Spec.packet = packet'';
+            Spec.pn_offset = pn_offset;
+            Spec.pn_len = pn_len;
+          })
+        end
+
+#push-options "--z3rlimit 256"
+
+#restart-solver
+
+let header_decrypt_aux_ct_correct
+  (a:ea)
+  (hpk: SCipher.key (SAEAD.cipher_alg_of_supported_alg a))
+  (cid_len: nat { cid_len <= 20 })
+  (packet: packet)
+: Lemma
+  (header_decrypt_aux_ct a hpk cid_len packet == Spec.header_decrypt_aux a hpk cid_len packet)
+= 
+  let open FStar.Math.Lemmas in
+  if Seq.length packet = 0
+  then ()
+  else
+    let f = Seq.index packet 0 in
+    let is_short = (BF.get_bitfield (U8.v f) 7 8 = 0) in
+    let is_retry = not is_short && BF.get_bitfield (U8.v f) 4 6 = 3 in
+    if is_retry
+    then ()
+    else
+      match Parse.putative_pn_offset cid_len packet with
+      | None -> ()
+      | Some pn_offset ->
+        let sample_offset = pn_offset + 4 in
+        if sample_offset + 16 > Seq.length packet
+        then ()
+        else begin
+          let sample = Seq.slice packet sample_offset (sample_offset+16) in
+          let mask = Seq.seq_reveal #Secret.U8 (Spec.block_of_sample (SAEAD.cipher_alg_of_supported_alg a) hpk (Seq.seq_hide #Secret.U8 sample)) in
+          (* mask the least significant bits of the first byte *)
+          let protected_bits = if is_short then 5 else 4 in
+          let f' = BF.set_bitfield (U8.v f) 0 protected_bits (BF.get_bitfield (U8.v f `FStar.UInt.logxor` U8.v (Seq.index mask 0)) 0 protected_bits) in
+          let packet' = Seq.cons (U8.uint_to_t f') (Seq.slice packet 1 (Seq.length packet)) in
+          (* now the packet number length is available, so mask the packet number *)
+          let pn_len = BF.get_bitfield f' 0 2 in
+          let pnmask_ct = Lemmas.and_inplace (Seq.slice mask 1 5) (pn_sizemask_ct pn_len) 0 in
+          let pnmask_naive = Lemmas.and_inplace (Seq.slice mask 1 (pn_len + 2)) (Spec.pn_sizemask pn_len) 0 in
+          Lemmas.pointwise_op_split U8.logand (Seq.slice mask 1 5) (pn_sizemask_ct pn_len) 0 (pn_len + 1);
+          assert (pnmask_naive `Seq.equal` Seq.slice pnmask_ct 0 (pn_len + 1));
+          let r = packet' in
+          Seq.lemma_split r (pn_offset + pn_len + 1);
+          Lemmas.pointwise_op_split U8.logxor r pnmask_ct pn_offset (pn_offset + pn_len + 1);
+          Lemmas.pointwise_op_split U8.logxor r pnmask_naive pn_offset (pn_offset + pn_len + 1);
+          Lemmas.pointwise_op_empty U8.logxor (Seq.slice r (pn_offset + pn_len + 1) (Seq.length r)) (Seq.slice pnmask_naive (pn_len + 1) (Seq.length pnmask_naive)) 0;
+          Lemmas.xor_inplace_zero (Seq.slice r (pn_offset + pn_len + 1) (Seq.length r)) (Seq.slice pnmask_ct (pn_len + 1) 4)
+            (fun i ->
+              Lemmas.and_inplace_zero
+                (Seq.slice mask (pn_len + 2) 5)
+                (Seq.slice (pn_sizemask_ct pn_len) (pn_len + 1) 4)
+                (fun j -> index_pn_sizemask_ct_right pn_len (j + (pn_len + 1)))
+                i
+            )
+            0
+        end
+
+#pop-options
+
+#restart-solver
+
+let header_decrypt_aux_ct_secret_preserving_not_retry_spec
+  (a:ea)
+  (hpk: SCipher.key (SAEAD.cipher_alg_of_supported_alg a))
+  (cid_len: nat { cid_len <= 20 })
+  (packet: Seq.seq Secret.uint8 { 
+    let l = Seq.length packet in
+    0 < l /\ l < pow2 32
+  })
+  (is_short: bool {
+    let i = Secret.v #Secret.U8 (Seq.index packet 0) in
+    (is_short == true <==> BF.get_bitfield #8 i 7 8 == 0) /\
+    (~ (not is_short && BF.get_bitfield #8 i 4 6 = 3))
+  })
+  (pn_offset: nat {
+    match Parse.putative_pn_offset cid_len (Seq.seq_reveal packet) with
+    | None -> False
+    | Some pn_offset' ->
+      pn_offset == pn_offset' /\
+      pn_offset + 20 <= Seq.length packet
+  })
+  : GTot (Spec.header_decrypt_aux_t)
+=
+  let f = Seq.index packet 0 in
+  let sample_offset = pn_offset + 4 in
+  let sample = Seq.slice packet sample_offset (sample_offset+16) in
+  let mask = Spec.block_of_sample (SAEAD.cipher_alg_of_supported_alg a) hpk sample in
+  (* mask the least significant bits of the first byte *)
+  let protected_bits = if is_short then 5ul else 4ul in
+  let f' = Secret.set_bitfield f 0ul protected_bits (Secret.get_bitfield (f `Secret.logxor` (Seq.index mask 0)) 0ul protected_bits) in
+  let packet' = Seq.cons f' (Seq.slice packet 1 (Seq.length packet)) in
+  (* now the packet number length is available, so mask the packet number *)
+  let pn_len = Secret.get_bitfield f' 0ul 2ul in
+  let pnmask = Lemmas.secret_and_inplace (Seq.slice mask 1 5) (Seq.seq_hide #Secret.U8 (pn_sizemask_ct (Secret.v pn_len))) 0 in
+  let packet'' = Lemmas.secret_xor_inplace packet' pnmask pn_offset in
+  {
+    Spec.is_short = is_short;
+    Spec.is_retry = false;
+    Spec.packet = Seq.seq_reveal #Secret.U8 packet'';
+    Spec.pn_offset = pn_offset;
+    Spec.pn_len = Secret.v pn_len;
+  }
+
+let header_decrypt_aux_ct_secret_preserving_not_retry_spec_correct
+  (a:ea)
+  (hpk: SCipher.key (SAEAD.cipher_alg_of_supported_alg a))
+  (cid_len: nat { cid_len <= 20 })
+  (packet: Seq.seq Secret.uint8 { 
+    let l = Seq.length packet in
+    0 < l /\ l < pow2 32
+  })
+  (is_short: bool {
+    let i = Secret.v #Secret.U8 (Seq.index packet 0) in
+    (is_short == true <==> BF.get_bitfield #8 i 7 8 == 0) /\
+    (~ (not is_short && BF.get_bitfield #8 i 4 6 = 3))
+  })
+  (pn_offset: nat {
+    match Parse.putative_pn_offset cid_len (Seq.seq_reveal packet) with
+    | None -> False
+    | Some pn_offset' ->
+      pn_offset == pn_offset' /\
+      pn_offset + 20 <= Seq.length packet
+  })
+: Lemma
+  (header_decrypt_aux_ct a hpk cid_len (Seq.seq_reveal packet) == Some (header_decrypt_aux_ct_secret_preserving_not_retry_spec a hpk cid_len packet is_short pn_offset))
+= assert (Some? (header_decrypt_aux_ct a hpk cid_len (Seq.seq_reveal packet)));
+  assume False
+
+inline_for_extraction
+let header_decrypt_aux_ct_secret_preserving_not_retry'
+  (a: ea)
+  (s: CTR.state (SAEAD.cipher_alg_of_supported_alg a))
+  (k: B.buffer Secret.uint8)
+  (cid_len: short_dcid_len_t)
+  (is_short: bool)
+  (pn_offset: U32.t)
+  (dst: B.buffer Secret.uint8)
+: HST.Stack unit
+  (requires (fun m ->
+    let l = B.length dst in
+    B.all_live m [B.buf k; B.buf dst] /\
+    CTR.invariant m s /\
+    B.length k == SCipher.key_length (SAEAD.cipher_alg_of_supported_alg a) /\
+    B.all_disjoint
+      [ CTR.footprint m s; B.loc_buffer k; B.loc_buffer dst] /\
+    0 < l /\ l < pow2 32 /\ (
+    let i = Secret.v #Secret.U8 (Seq.index (B.as_seq m dst) 0) in
+    (is_short == true <==> BF.get_bitfield #8 i 7 8 == 0) /\
+    (~ (not is_short && BF.get_bitfield #8 i 4 6 = 3)) /\ (
+    match Parse.putative_pn_offset (U32.v cid_len) (Seq.seq_reveal (B.as_seq m dst)) with
+    | None -> False
+    | Some pn_offset' ->
+      U32.v pn_offset == pn_offset' /\
+      pn_offset' + 20 <= l
+  ))))
+  (ensures (fun m _ m' ->
+    B.modifies (B.loc_buffer dst `B.loc_union` CTR.footprint m s) m m' /\
+    CTR.invariant m' s /\
+    CTR.footprint m s == CTR.footprint m' s /\
+    (header_decrypt_aux_ct_secret_preserving_not_retry_spec a (B.as_seq m k) (U32.v cid_len) (B.as_seq m dst) is_short (U32.v pn_offset)).Spec.packet == Seq.seq_reveal (B.as_seq m' dst)
+  ))
+= admit ()
+
+#push-options "--z3rlimit 32 --query_stats"
+
+#restart-solver
+
+let header_decrypt_aux_ct_secret_preserving_not_retry
+  (a: ea)
+  (s: CTR.state (SAEAD.cipher_alg_of_supported_alg a))
+  (k: B.buffer Secret.uint8)
+  (cid_len: short_dcid_len_t)
+  (is_short: bool)
+  (pn_offset: U32.t)
+  (dst: B.buffer U8.t)
+: HST.Stack unit
+  (requires (fun m ->
+    let l = B.length dst in
+    B.all_live m [B.buf k; B.buf dst] /\
+    CTR.invariant m s /\
+    B.length k == SCipher.key_length (SAEAD.cipher_alg_of_supported_alg a) /\
+    B.all_disjoint
+      [ CTR.footprint m s; B.loc_buffer k; B.loc_buffer dst] /\
+    0 < l /\ l < pow2 32 /\ (
+    let i = Secret.v #Secret.U8 (Seq.index (B.as_seq m dst) 0) in
+    (is_short == true <==> BF.get_bitfield #8 i 7 8 == 0) /\
+    (~ (not is_short && BF.get_bitfield #8 i 4 6 = 3)) /\ (
+    match Parse.putative_pn_offset (U32.v cid_len) (B.as_seq m dst) with
+    | None -> False
+    | Some pn_offset' ->
+      U32.v pn_offset == pn_offset' /\
+      pn_offset' + 20 <= l
+  ))))
+  (ensures (fun m _ m' ->
+    match Spec.header_decrypt_aux a (B.as_seq m k) (U32.v cid_len) (B.as_seq m dst) with
+    | None -> False
+    | Some res ->
+      let len_mod = U32.v pn_offset + res.Spec.pn_len + 1 in
+      res.Spec.pn_offset == U32.v pn_offset /\
+      len_mod <= B.length dst /\
+      B.modifies (B.loc_buffer (B.gsub dst 0ul (U32.uint_to_t len_mod)) `B.loc_union` CTR.footprint m s) m m' /\
+      CTR.invariant m' s /\
+      CTR.footprint m s == CTR.footprint m' s /\
+      res.Spec.packet == B.as_seq m' dst
+  ))
+=
+  let m = HST.get () in
+  SecretBuffer.with_whole_buffer_hide_weak_modifies
+    #unit
+    dst
+    m
+    (CTR.footprint m s `B.loc_union` B.loc_buffer k)
+    (CTR.footprint m s)
+    true
+    (fun _ cont m' ->
+      (header_decrypt_aux_ct_secret_preserving_not_retry_spec a (B.as_seq m k) (U32.v cid_len) (Seq.seq_hide #Secret.U8 (B.as_seq m dst)) is_short (U32.v pn_offset)).Spec.packet == cont /\
+      CTR.invariant m' s /\
+      CTR.footprint m s == CTR.footprint m' s
+    )
+    (fun _ bs ->
+      header_decrypt_aux_ct_secret_preserving_not_retry' a s k cid_len is_short pn_offset bs
+    );
+  let m' = HST.get () in
+  header_decrypt_aux_ct_secret_preserving_not_retry_spec_correct a (B.as_seq m k) (U32.v cid_len) (Seq.seq_hide #Secret.U8 (B.as_seq m dst)) is_short (U32.v pn_offset);
+  header_decrypt_aux_ct_correct a (B.as_seq m k) (U32.v cid_len) (B.as_seq m dst);
+  Spec.header_decrypt_aux_post a (B.as_seq m k) (U32.v cid_len) (B.as_seq m dst);
+  let len_mod = Ghost.hide (U32.uint_to_t (U32.v pn_offset + (Some?.v (Spec.header_decrypt_aux a (B.as_seq m k) (U32.v cid_len) (B.as_seq m dst))).Spec.pn_len + 1)) in
+  B.modifies_loc_buffer_from_to_intro dst 0ul len_mod (CTR.footprint m s) m m'
+
+#pop-options
+
+let header_decrypt_aux
+  (a: ea)
+  (s: CTR.state (SAEAD.cipher_alg_of_supported_alg a))
+  (k: B.buffer Secret.uint8)
+  (cid_len: short_dcid_len_t)
+  (dst: B.buffer U8.t)
+  (dst_len: U32.t)
+: HST.Stack bool
+  (requires (fun m ->
+    let l = B.length dst in
+    B.all_live m [B.buf k; B.buf dst] /\
+    CTR.invariant m s /\
+    B.length k == SCipher.key_length (SAEAD.cipher_alg_of_supported_alg a) /\
+    B.all_disjoint
+      [ CTR.footprint m s; B.loc_buffer k; B.loc_buffer dst] /\
+    B.length dst == U32.v dst_len
+  ))
+  (ensures (fun m res m' ->
+    CTR.invariant m' s /\
+    CTR.footprint m s == CTR.footprint m' s /\ (
+    match res, Spec.header_decrypt_aux a (B.as_seq m k) (U32.v cid_len) (B.as_seq m dst) with
+    | false, None ->
+      B.modifies B.loc_none m m'
+    | true, Some res ->
+      res.Spec.packet == B.as_seq m' dst /\
+      (if res.Spec.is_retry
+      then B.modifies B.loc_none m m'
+      else
+        let len = res.Spec.pn_offset + res.Spec.pn_len + 1 in
+        len <= B.length dst /\
+        B.modifies (CTR.footprint m s `B.loc_union` B.loc_buffer (B.gsub dst 0ul (U32.uint_to_t len))) m m'
+      )
+    | _ -> False
+  )))
+= let m = HST.get () in
+  if dst_len = 0ul
+  then false
+  else
+    let f = B.index dst 0ul in
+    let isshort = BF.uint8.BF.get_bitfield f 7 8 = 0uy in
+    let isretry = not isshort && (BF.uint8.BF.get_bitfield f 4 6 = 3uy) in
+    if isretry
+    then true
+    else match ParseImpl.putative_pn_offset cid_len dst dst_len with
+    | None -> false
+    | Some pn_offset ->
+      if dst_len `U32.lt` (pn_offset `U32.add` 20ul)
+      then false
+      else begin
+        header_decrypt_aux_ct_secret_preserving_not_retry a s k cid_len isshort pn_offset dst;
+        true
+      end
 
 (*
 
@@ -470,7 +810,7 @@ header_encrypt_ct_secret_preserving_not_retry_spec_correct
 : HST.Stack unit
   (requires (fun m ->
     B.live m b /\
-    B.as_seq m b == ParseSpec.format_header h `Seq.append` c
+    B.as_seq m b == Parse.format_header h `Seq.append` c
   ))
   (ensures (fun m _ m' ->
     B.modifies (B.loc_buffer b)
